Current status of RC formalization.

Semantics.v
@@ -1,217 +1,12 @@
 Require Import Lists.List Lists.ListSet Vector Arith.PeanoNat Syntax AbstractRelation Bool.Sumbool Tribool JMeq 
-  FunctionalExtensionality ProofIrrelevance Eqdep_dec EqdepFacts Omega Util RelFacts.
+  FunctionalExtensionality ProofIrrelevance Eqdep_dec EqdepFacts Omega Util RelFacts Common Eval.
 
-Module Type EV (Db : DB) (Sql : SQL Db).
-
+Module SQLSemantics (Db : DB) (Sem: SEM Db) (Sql : SQL Db).
   Import Db.
+  Import Sem.
   Import Sql.
-
-  Parameter preenv : Type.  (* environment (for evaluation) *)
-  Parameter env : Ctx -> Type.
-  Parameter env_lookup  : forall G : Ctx, env G -> FullVar -> option Value.
-
-  Parameter j_tm_sem : forall G, pretm -> (env G -> Value) -> Prop.
-  Parameter j_tml_sem : forall G (tml : list pretm), (env G -> Rel.T (List.length tml)) -> Prop.
-
-  Hypothesis j_tm_sem_fun :
-    forall G t St, j_tm_sem G t St -> forall St0, j_tm_sem G t St0 -> St = St0.
-  Hypothesis j_tml_sem_fun :
-    forall G tml Stml, j_tml_sem G tml Stml -> forall Stml0, j_tml_sem G tml Stml0 -> Stml = Stml0.
-
-  Hypothesis env_of_tuple : forall G, forall Vl : Db.Rel.T (list_sum (List.map (List.length (A:=Name)) G)), env G.
-
-  Hypothesis length_tmlist : forall c0, length (tmlist_of_ctx c0) = length (concat c0).
-  Hypothesis length_tolist : forall A n (v : Vector.t A n), length (to_list v) = n.
-
-  Parameter Vector_combine : forall A B n, Vector.t A n -> Vector.t B n -> Vector.t (A * B) n.
-
-  Hypothesis env_app : forall G1 G2, env G1 -> env G2 -> env (G1++G2).
-
-End EV.
-
-Fixpoint findpos {A} (l : list A) (p : A -> bool) start {struct l} : option nat := 
-  match l with
-  | List.nil => None
-  | List.cons a l0 => if p a then Some start else findpos l0 p (S start)
-  end.
-
-Module Evl (Db : DB) (Sql : SQL Db) <: EV Db Sql.
-  Import Db.
-  Import Sql.
-
-  Definition preenv := list Value. (* environment (for evaluation) *)
-  Definition env := fun (g : Ctx) => 
-    { h : preenv & (List.length (List.concat g) =? List.length h) = true }. 
-
-  Fixpoint scm_env s (h : preenv) {struct s} : list (Name * Value) * preenv := 
-    match s, h with
-    | List.nil, _ => (List.nil, h)
-    | _, List.nil => (List.nil, List.nil)
-    | a::s0, v::h0 => let (sh,h') := scm_env s0 h0 in ((a,v)::sh,h')
-    end. 
-
-  Fixpoint ctx_env G (h : preenv) {struct G} : list (list (Name * Value)) :=
-    match G with
-    | List.nil => List.nil
-    | s::G0 => let (sh,h') := scm_env s h in sh :: ctx_env G0 h'
-    end.
-
-  Definition env_lookup : forall G : Ctx, env G -> FullVar -> option Value :=
-    fun G h x => let (n,a) := x in
-      bind (nth_error (ctx_env G (projT1 h)) n)
-        (fun sh => bind (find (fun x => if Db.Name_dec (fst x) a then true else false) sh)
-          (fun p => ret (snd p))).
-
-  Lemma findpos_Some A (s : list A) p :
-    forall m n, findpos s p m = Some n -> n < m + length s.
-  Proof.
-    elim s; simpl; intros; intuition.
-    + discriminate H.
-    + destruct (p a); intuition.
-      - injection H0. omega. 
-      - pose (H _ _ H0). omega.
-  Qed.
-
-  Lemma j_var_nth_aux (h : list Value) s a : forall i,
-    findpos s (fun x => if Db.Name_dec x a then true else false) 0 = Some i ->
-    length s = length h ->
-    { v : Value & nth_error h i = Some v }.
-  Proof.
-    intros. cut (nth_error h i <> None).
-    + destruct (nth_error h i); intuition. exists v; reflexivity.
-    + apply nth_error_Some. rewrite <- H0. pose (findpos_Some _ _ _ _ _ H). omega.
-  Qed.
-
-  Lemma nth_error_map A B n a (f : A -> B) : 
-    forall (l : list A), nth_error l n = Some a ->
-    nth_error (List.map f l) n = Some (f a).
-  Proof.
-    elim n; simpl.
-    + intro l; destruct l; simpl; intuition.
-      - discriminate H.
-      - injection H. intro. rewrite H0. reflexivity.
-    + intros m IH l; destruct l; simpl; intuition. discriminate H.
-  Qed.
-
-  Lemma nth_error_map_r A B n b (f : A -> B) : 
-    forall (l : list A), nth_error (List.map f l) n = Some b ->
-    { a : A & nth_error l n = Some a /\ b = f a }.
-  Proof.
-    elim n; simpl.
-    + intro l; destruct l; simpl; intuition.
-      - discriminate H.
-      - injection H. intro. exists a. rewrite H0. auto.
-    + intros m IH l; destruct l; simpl; intuition. discriminate H.
-  Qed.
-
-(*
-  Lemma env_scm_length (G : Ctx) (h : env G) : forall n s, 
-    List.nth_error G n = Some s -> { h0 : list Value & List.nth_error (projT1 h) n = Some h0 /\ length s = length h0 }.
-  Proof.
-    intros. destruct h. pose (nth_error_map _ _ _ _ (@length Name) _ H).
-    clearbody e0. rewrite e in e0. destruct (nth_error_map_r _ _ _ _ _ _ e0).
-    destruct a. exists x0. simpl. auto.
-  Qed.
-*)
-
-  Definition unopt {A} : forall (x : option A), x <> None -> A.
-    refine (fun x => match x as x0 return (x0 <> None -> A) with Some x' => fun _ => x' | None => _ end).
-    intro Hfalse. contradiction Hfalse. reflexivity.
-  Defined.
-
-  Lemma unopt_pi {A} (x : option A) Hx Hx' : unopt x Hx = unopt x Hx'.
-  Proof.
-    destruct x; intuition.
-    contradiction Hx. reflexivity.
-  Qed.
-
-  Lemma p_scm_preenv s G (h : preenv) :
-    length h = length (List.concat (s::G)) ->
-    forall y h0, scm_env s h = (y,h0) ->
-    length y = length s /\ length h0 = length h - length s.
-  Proof.
-    intros. generalize s, H, y, h0, H0. clear s H y h0 H0. induction h; simpl; intros.
-    + destruct s.
-      - simpl in H0. injection H0. intros. subst. intuition.
-      - simpl in H. discriminate H.
-    + destruct s.
-      - simpl. simpl in H0. injection H0; intros; subst. simpl; intuition.
-      - simpl in H0. destruct (scm_env s h) eqn:e0. injection H0; intros; clear H0. 
-        simpl in H. injection H. intro. clear H.
-        destruct (IHh _ H0 _ _ e0). subst. split.
-        * simpl. rewrite H. reflexivity.
-        * rewrite H3. simpl. reflexivity.
-  Qed.
-
-  Lemma p_scm_env s G (h : env (s::G)) :
-    forall y p, scm_env s (projT1 h) = (y,p) ->
-    length y = length s /\ length p = length (projT1 h) - length s.
-  Proof.
-    intros. destruct h. simpl in e. eapply (p_scm_preenv _ G). symmetry.
-    apply Nat.eqb_eq. exact e. exact H.
-  Qed.
-
-  Definition env_hd {a} {s} {G} : env ((a::s)::G) -> Value.
-    refine (fun h => unopt (List.hd_error (projT1 h)) _).
-    destruct h. simpl. destruct x; simpl; intuition. discriminate H.
-  Defined.
-
-  Definition env_tl {a} {s} {G} : env ((a::s)::G) -> env (s::G).
-    refine (fun h => _).
-    enough ((length (concat (s::G)) =? length (List.tl (projT1 h))) = true).
-    unfold env. econstructor. exact H.
-    destruct h. destruct x; simpl; intuition.
-  Defined.
-
-  Inductive j_var_sem : forall s, Name -> (env (s::List.nil) -> Value) -> Prop :=
-  | jvs_hd : forall a s, ~ List.In a s -> j_var_sem (a::s) a (fun h => env_hd h)
-  | jvs_tl : forall a s b, 
-      forall Sb, a <> b -> j_var_sem s b Sb -> j_var_sem (a::s) b (fun h => Sb (env_tl h)).
-
-  Theorem j_var_sem_fun :
-    forall s a Sa, j_var_sem s a Sa -> forall Sa0, j_var_sem s a Sa0 -> Sa = Sa0.
-  Proof.
-    intros s a Sa Ha. induction Ha.
-    + intros. inversion H0.
-      - apply (existT_eq_elim H5). intros _. apply JMeq_eq.
-      - contradiction H5. reflexivity.
-    + intros. inversion H0.
-      - contradiction H.
-      - apply (existT_eq_elim H3); clear H3; intros; subst.
-        rewrite (IHHa _ H6). reflexivity.
-  Qed.
-
-  Definition subenv1 {G1} {G2} : env (G1++G2) -> env G1.
-    refine (fun h => _).
-    enough ((length (concat G1) =? length (firstn (length (concat G1)) (projT1 h))) = true).
-    unfold env. econstructor. exact H.
-    destruct h. apply Nat.eqb_eq. symmetry. apply firstn_length_le.
-    simpl. rewrite <- (proj1 (Nat.eqb_eq _ _) e). rewrite concat_app. rewrite app_length. omega.
-  Defined.
-
-  Definition subenv2 {G1} {G2} : env (G1++G2) -> env G2.
-    refine (fun h => _).
-    enough ((length (concat G2) =? length (skipn (length (concat G1)) (projT1 h))) = true).
-    unfold env. econstructor. exact H.
-    destruct h. apply Nat.eqb_eq. simpl. rewrite length_skipn.
-    rewrite <- (proj1 (Nat.eqb_eq _ _) e). rewrite concat_app. rewrite app_length. omega.
-  Defined.
-
-  Inductive j_fvar_sem : forall G, nat -> Name -> (env G -> Value) -> Prop :=
-  | jfs_hd : forall s G a, 
-      forall Sa, j_var_sem s a Sa -> j_fvar_sem (s::G) O a (fun h => Sa (@subenv1 (s::List.nil) G h))
-  | jfs_tl : forall s G i a,
-      forall Sia, j_fvar_sem G i a Sia -> j_fvar_sem (s::G) (S i) a (fun h => Sia (@subenv2 (s::List.nil) G h)).
-
-  Theorem j_fvar_sem_fun :
-    forall G i a Sia, j_fvar_sem G i a Sia -> forall Sia0, j_fvar_sem G i a Sia0 -> Sia = Sia0.
-  Proof.
-    intros G i a Sia Hia. induction Hia.
-    + intros. inversion H0. apply (existT_eq_elim H2); clear H2; intros; subst. clear H2.
-      rewrite (j_var_sem_fun _ _ _ H _ H5). reflexivity.
-    + intros. inversion H. apply (existT_eq_elim H5); clear H5; intros; subst.
-      rewrite (IHHia _ H4). reflexivity.
-  Qed.
+  Module Ev := Evl Db.
+  Import Ev.
 
   Inductive j_tm_sem0 (G:Ctx) : pretm -> (env G -> Value) -> Prop :=
   | jts_const : forall c, j_tm_sem0 G (tmconst c) (fun _ => Db.c_sem c)
@@ -227,6 +22,7 @@ Module Evl (Db : DB) (Sql : SQL Db) <: EV Db Sql.
       j_tm_sem0 G t St -> j_tml_sem0 G tml Stml ->
       j_tml_sem0 G (t::tml) (fun h => Vector.cons _ (St h) _ (Stml h)).
 
+  Derive Inversion j_tml_nil_sem with (forall G S, j_tml_sem0 G List.nil S).
   Derive Inversion j_tml_cons_sem with (forall G t tml Stml, j_tml_sem0 G (t::tml) Stml) Sort Prop.
 
   (* we need to fool the kernel, because it doesn't accept instantiation to inductive types *)
@@ -251,134 +47,6 @@ Module Evl (Db : DB) (Sql : SQL Db) <: EV Db Sql.
       rewrite (j_tm_sem_fun _ _ _ H _ H3). rewrite (IHHtml _ H5). reflexivity.
   Qed.
 
-  Definition env_app : forall G1 G2, env G1 -> env G2 -> env (G1++G2).
-    refine (fun G1 G2 h1 h2 => existT _ (projT1 h1 ++ projT1 h2) _).
-    destruct h1. destruct h2. apply Nat.eqb_eq. 
-    rewrite concat_app. simpl. do 2 rewrite app_length. 
-    f_equal; apply Nat.eqb_eq.
-    exact e.
-    exact e0.
-  Defined.
-
-  Fixpoint env_of_tuple G : Db.Rel.T (list_sum (List.map (List.length (A:=Name)) G)) -> env G.
-    refine 
-      ((match G as G0 return (G = G0 -> Db.Rel.T (list_sum (List.map (@length Name) G0)) -> env G0) with
-      | List.nil => _
-      | List.cons s G1 => _
-      end) eq_refl).
-    + refine (fun _ _ => existT _ List.nil _). reflexivity.
-    + simpl. intros. pose (p := split X); clearbody p.
-      apply (env_app (s :: List.nil)).
-      - eapply (existT _ (Vector.to_list (fst p)) _). Unshelve. simpl.
-        rewrite length_to_list. rewrite app_length. simpl. apply Nat.eqb_eq. omega.
-      - apply (env_of_tuple _ (snd p)).
-  Defined.
-
-  Definition Vector_combine {A} {B} {n} : Vector.t A n -> Vector.t B n -> Vector.t (A * B) n :=
-    Vector.rect2 (fun n0 _ _ => Vector.t (A*B) n0) (Vector.nil _)
-    (fun m _ _ acc a b => Vector.cons _ (a,b) _ acc).
-
-  Lemma length_tmlist c0 : length (tmlist_of_ctx c0) = length (concat c0).
-  Proof.
-    unfold tmlist_of_ctx. unfold mapi. generalize 0.
-    elim c0; intuition. 
-    simpl. do 2 rewrite app_length. rewrite cmap_length.
-    f_equal. apply H.
-  Qed.
-
-  Lemma length_tolist A n (v : Vector.t A n): length (to_list v) = n.
-  Proof.
-    elim v; simpl; intuition.
-  Qed.
-
-  Lemma nth_error_app2_eq {A} (G2:list A) n : forall G1, nth_error (G2 ++ G1) (length G2 + n) = nth_error G1 n.
-  Proof.
-    elim G2; auto.
-  Qed.
-
-  Lemma scm_env_skipn s : forall l h h0, scm_env s h = (l, h0) -> h0 = skipn (length s) h.
-  Proof.
-    induction s.
-    + simpl; intros. injection H; intuition.
-    + intros. destruct h.
-      - simpl in H. simpl. injection H; intuition.
-      - simpl in H. simpl. destruct (scm_env s h) eqn:e. injection H. intros. 
-        subst. apply (IHs _ _ _ e).
-  Qed.
-
-  Lemma skipn_skipn {A} m n : forall (l : list A), skipn m (skipn n l) = skipn (m+n) l.
-  Proof.
-    induction n.
-    + simpl; intuition. replace (m + 0) with m. reflexivity. omega.
-    + intro. destruct l.
-      - simpl. destruct m; simpl; intuition.
-      - replace (m + S n) with (S (m + n)). simpl. apply IHn.
-        omega.
-  Qed.
-
-  Lemma skipn_append {A} (l1 l2 : list A) : skipn (length l1) (l1 ++ l2) = l2.
-  Proof.
-    induction l1; simpl; intuition.
-  Qed.
-
-  Lemma nth_error_ctx_env_app_eq G2 n : forall G1 h1 h2,
-      length (concat G1) = length h1 ->
-      length (concat G2) = length h2 ->
-      nth_error (ctx_env (G2 ++ G1) (h2 ++ h1)) (length G2 + n)
-      = nth_error (ctx_env G1 h1) n.
-  Proof.
-    induction G2; simpl; intuition.
-    + replace h2 with (@List.nil Value). reflexivity.
-      symmetry. apply length_zero_iff_nil. intuition.
-    + destruct (scm_env a (h2++h1)) eqn:e. rewrite app_length in H0.
-      enough (length (h2++h1) = length (List.concat (a::G2++G1))).
-      destruct (p_scm_preenv _ _ _ H1 _ _ e).
-      simpl in H1. rewrite concat_app in H1. repeat rewrite app_length in H1.
-      enough (length p = length (concat G2) + length (concat G1)).
-      rewrite <- (firstn_skipn (length (concat G2)) p).
-      replace (skipn (length (concat G2)) p) with h1.
-      apply IHG2. exact H. rewrite firstn_length. rewrite H4. rewrite min_l. reflexivity. omega.
-      rewrite (scm_env_skipn _ _ _ _ e). 
-      rewrite skipn_skipn. 
-      replace (length (concat G2) + length a) with (length h2). symmetry. apply skipn_append.
-      omega.
-      rewrite H3. rewrite app_length. omega.
-      simpl. rewrite concat_app. do 3 rewrite app_length. omega.
-  Qed.
-
-  Lemma length_env {G} (h: env G) : length (projT1 h) = length (concat G).
-  Proof.
-    destruct h. simpl. symmetry. apply Nat.eqb_eq. exact e.
-  Qed.
-
-  Definition env_of_list (G:Ctx) : forall (l: list Value), length l = length (List.concat G) -> env G.
-    intros. exists l. apply Nat.eqb_eq. intuition.
-  Defined.
-
-  Lemma bool_eq_pi : forall (b1 b2 : bool) (e1 e2 : b1 = b2), e1 = e2.
-  Proof.
-    intros b1 b2. enough (forall (x y : bool), x = y \/ x <> y).
-    destruct b1, b2. 
-    + intro. eapply (K_dec H (fun e => forall e2 : true = true, e = e2) _ e1). Unshelve.
-      simpl. intro. eapply (K_dec H (fun e => eq_refl = e) _ e2). Unshelve. reflexivity.
-    + intros. discriminate e1.
-    + intros. discriminate e1.
-    + intro. eapply (K_dec H (fun e => forall e2 : false = false, e = e2) _ e1). Unshelve.
-      simpl. intro. eapply (K_dec H (fun e => eq_refl = e) _ e2). Unshelve. reflexivity.
-    + intros. destruct (Bool.bool_dec x y); intuition.
-  Qed.
-
-  Lemma env_eq {G} (h1 h2: env G) : projT1 h1 = projT1 h2 -> h1 = h2.
-  Proof.
-    destruct h1. destruct h2. simpl. intro. subst. f_equal. apply bool_eq_pi.
-  Qed.
-
-  Lemma env_JMeq {G1} {G2} (h1: env G1) (h2: env G2): G1 = G2 -> projT1 h1 = projT1 h2 -> h1 ~= h2.
-  Proof.
-    intro. subst.
-    destruct h1. destruct h2. simpl. intro. subst. apply eq_JMeq. f_equal. apply bool_eq_pi.
-  Qed.
-
   Lemma j_tm_sem_weak G G' t St (Ht : j_tm_sem G t St) :
     j_tm_sem (G' ++ G) (tm_lift t (length G')) (fun h => St (subenv2 h)).
   Proof.
@@ -398,170 +66,40 @@ Module Evl (Db : DB) (Sql : SQL Db) <: EV Db Sql.
     induction H; constructor; intuition.
   Qed.
 
-End Evl.
+  (* alternate -- not stronger but easier -- version of sum *)
 
-Module Type SEM (Db : DB).
-  Import Db.
-  Parameter B : Type.
-  Parameter btrue : B.
-  Parameter bfalse : B.
-  Parameter bmaybe : B.
-  Parameter band : B -> B -> B.
-  Parameter bor : B -> B -> B.
-  Parameter bneg : B -> B.
-  Parameter is_btrue : B -> bool.
-  Parameter is_bfalse : B -> bool.
-  Parameter of_bool : bool -> B.
-  Parameter veq : Value -> Value -> B.
+  Axiom R_sum : forall m n, Rel.R m -> (Rel.T m -> Rel.R n) -> Rel.R n.
+  Implicit Arguments R_sum [m n].
 
-  Hypothesis sem_bpred : forall n, (forall l : list BaseConst, length l = n -> bool) -> 
-    forall l : list Value, length l = n -> B.
+  (* singleton rel *)
+  Definition R_single {m} : Rel.T m -> Rel.R m :=
+    fun t => Rel.sum Rel.Rone (fun _ => t).
 
-  Hypothesis sem_bpred_elim : 
-    forall n (p : forall l, length l = n -> bool) (l : list Value) (Hl : length l = n) (P : B -> Prop),
-    (forall cl, monadic_map (fun val => val) l = Some cl -> forall Hcl : length cl = n, P (of_bool (p cl Hcl))) ->
-    (monadic_map (fun val => val) l = None -> P bmaybe) ->
-    P (sem_bpred n p l Hl).
-End SEM.
 
-Module Sem2 (Db : DB) <: SEM Db.
-  Import Db.
-  Definition B := bool.
-  Definition btrue := true.
-  Definition bfalse := false.
-  Definition bmaybe := false.
-  Definition band := andb.
-  Definition bor := orb.
-  Definition bneg := negb.
-  Definition is_btrue := fun (x : bool) => x.
-  Definition is_bfalse := fun (x : bool) => negb x.
-  Definition of_bool := fun (x : bool) => x.
-  Definition veq := fun v1 v2 => 
-    match v1, v2 with
-    | Some x1, Some x2 => c_eq x1 x2
-    | _, _ => false
-    end.
-
-  Definition sem_bpred_aux
-  : forall n (p : (forall l : list BaseConst, length l = n -> bool)), 
-      forall (l : list Value), length l = n -> 
-      { b : B & (forall x Hx, monadic_map (fun val => val) l = Some x -> b = of_bool (p x Hx)) /\
-                (monadic_map (fun val => val) l = None -> b = false)}.
-  Proof.
-    intros n p l H.
-    destruct (monadic_map (fun val => val) l) eqn:e.
-    + eexists (of_bool (p l0 _)). Unshelve. Focus 2. 
-      rewrite <- (length_monadic_map _ _ _ _ _ e). exact H. split.
-      - intros. injection H0. intro. generalize Hx. clear Hx. rewrite <- H1.
-        intro. f_equal. f_equal. eapply UIP.
-      - intro Hfalse. discriminate Hfalse.
-    + exists false. split; intros.
-      - discriminate H0.
-      - reflexivity.
-  Defined.
-
-  Definition sem_bpred 
-  : forall n, (forall l : list BaseConst, length l = n -> bool) -> 
-      forall l : list Value, length l = n -> B :=
-  fun n p l H => projT1 (sem_bpred_aux n p l H).
-
-  Lemma sem_bpred_elim n (p : forall l, length l = n -> bool) (l : list Value) (Hl : length l = n) (P : B -> Prop) :
-    (forall cl, monadic_map (fun val => val) l = Some cl -> forall Hcl : length cl = n, P (of_bool (p cl Hcl))) ->
-    (monadic_map (fun val => val) l = None -> P false) ->
-    P (sem_bpred n p l Hl).
-  intros. cut ((forall x Hx, monadic_map (fun val => val) l = Some x -> sem_bpred n p l Hl = of_bool (p x Hx)) /\
-                (monadic_map (fun val => val) l = None -> sem_bpred n p l Hl = false)).
-  + intro Hcut. destruct Hcut. destruct (monadic_map (fun val => val) l) eqn:e; simpl.
-    - assert (length l0 = n). rewrite <- Hl. symmetry. apply (length_monadic_map _ _ _ _ _ e).
-      rewrite (H1 _ H3). apply H. reflexivity. reflexivity.
-    - rewrite (H2 eq_refl). apply H0. reflexivity.
-  + apply (projT2 (sem_bpred_aux n p l Hl)).
-  Qed.
-
-End Sem2.
-
-Module Sem3 (Db : DB) <: SEM Db.
-  Import Db.
-  Definition B := tribool.
-  Definition btrue := ttrue.
-  Definition bfalse := tfalse.
-  Definition bmaybe := unknown.
-  Definition band := andtb.
-  Definition bor := ortb.
-  Definition bneg := negtb.
-  Definition is_btrue := Tribool.eqb ttrue.
-  Definition is_bfalse := Tribool.eqb tfalse.
-  Definition of_bool := tribool_of_bool.
-  Definition veq := fun v1 v2 => 
-    match v1, v2 with
-    | Some x1, Some x2 => tribool_of_bool (c_eq x1 x2)
-    | _, _ => unknown
-    end.
-
-  Definition sem_bpred_aux
-  : forall n (p : (forall l : list BaseConst, length l = n -> bool)), 
-      forall (l : list Value), length l = n -> 
-      { b : B & (forall x Hx, monadic_map (fun val => val) l = Some x -> b = of_bool (p x Hx)) /\
-                (monadic_map (fun val => val) l = None -> b = unknown)}.
-  Proof.
-    intros n p l H.
-    destruct (monadic_map (fun val => val) l) eqn:e.
-    + eexists (of_bool (p l0 _)). Unshelve. Focus 2. 
-      rewrite <- (length_monadic_map _ _ _ _ _ e). exact H. split.
-      - intros. injection H0. intro. generalize Hx. clear Hx. rewrite <- H1.
-        intro. f_equal. f_equal. eapply UIP.
-      - intro Hfalse. discriminate Hfalse.
-    + exists unknown. split; intros.
-      - discriminate H0.
-      - reflexivity.
-  Defined.
-
-  Definition sem_bpred 
-  : forall n, (forall l : list BaseConst, length l = n -> bool) -> 
-      forall l : list Value, length l = n -> B :=
-  fun n p l H => projT1 (sem_bpred_aux n p l H).
-
-  Lemma sem_bpred_elim n (p : forall l, length l = n -> bool) (l : list Value) (Hl : length l = n) (P : B -> Prop) :
-    (forall cl, monadic_map (fun val => val) l = Some cl -> forall Hcl : length cl = n, P (of_bool (p cl Hcl))) ->
-    (monadic_map (fun val => val) l = None -> P unknown) ->
-    P (sem_bpred n p l Hl).
-  intros. cut ((forall x Hx, monadic_map (fun val => val) l = Some x -> sem_bpred n p l Hl = of_bool (p x Hx)) /\
-                (monadic_map (fun val => val) l = None -> sem_bpred n p l Hl = unknown)).
-  + intro Hcut. destruct Hcut. destruct (monadic_map (fun val => val) l) eqn:e; simpl.
-    - assert (length l0 = n). rewrite <- Hl. symmetry. apply (length_monadic_map _ _ _ _ _ e).
-      rewrite (H1 _ H3). apply H. reflexivity. reflexivity.
-    - rewrite (H2 eq_refl). apply H0. reflexivity.
-  + apply (projT2 (sem_bpred_aux n p l Hl)).
-  Qed.
-
-End Sem3.
-
-Module SQLSemantics (Db : DB) (Sem: SEM Db) (Sql : SQL Db) (Ev : EV Db Sql).
-  Import Db.
-  Import Sem.
-  Import Sql.
-  Import Ev.
-
+  (* NOTE: the ordering in the LATERAL list of lists grows dependencies left to right, while each of the 
+     inner lists has the same ordering (right to left) as contexts *)
   Inductive j_q_sem (d : Db.D) : forall G (s : Scm), prequery -> (env G -> Rel.R (List.length s)) -> Prop := 
-  | jqs_sel : forall G b tml btb c,
-      forall G0 Sbtb Sc Stml e,
-      j_btb_sem d G G0 btb Sbtb ->
+  | jqs_sel : forall G b tml btbl c,
+      forall G0 Sbtbl Sc Stml s e,
+      j_btbl_sem d G G0 btbl Sbtbl ->
       j_cond_sem d (G0++G) c Sc ->
-      j_tml_sem (G0++G) (List.map fst tml) Stml ->
-      j_q_sem d G (List.map snd tml) (select b tml btb c) 
-        (fun h => let S1 := Sbtb h in
+      j_tml_sem (G0++G) (List.map fst tml) Stml -> 
+      s = List.map snd tml ->
+      j_q_sem d G s (select b tml btbl c) 
+        (fun h => let S1 := Sbtbl h in
                   let p  := fun Vl => Sem.is_btrue (Sc (Ev.env_app _ _ (Ev.env_of_tuple G0 Vl) h)) in
                   let S2 := Rel.sel S1 p in
                   let f  := fun Vl => Stml (Ev.env_app _ _ (Ev.env_of_tuple G0 Vl) h) in
                   let S := cast _ _ e (Rel.sum S2 f)
                   in if b then Rel.flat S else S)
-  | jqs_selstar : forall G b btb c,
-      forall G0 Sbtb Sc Stml e,
-      j_btb_sem d G G0 btb Sbtb ->
+  | jqs_selstar : forall G b btbl c,
+      forall s0 G0 Sbtbl Sc Stml e,
+      j_btbl_sem d G G0 btbl Sbtbl ->
       j_cond_sem d (G0++G) c Sc ->
       j_tml_sem (G0++G) (tmlist_of_ctx G0) Stml ->
-      j_q_sem d G (List.concat G0) (selstar b btb c) 
-        (fun h => let S1 := Sbtb h in
+      s0 = List.concat G0 ->
+      j_q_sem d G s0 (selstar b btbl c) 
+        (fun h => let S1 := Sbtbl h in
                   let p  := fun Vl => Sem.is_btrue (Sc (Ev.env_app _ _ (Ev.env_of_tuple G0 Vl) h)) in
                   let S2 := Rel.sel S1 p in
                   let f  := fun Vl => Stml (Ev.env_app _ _ (Ev.env_of_tuple G0 Vl) h) in
@@ -637,25 +175,38 @@ Module SQLSemantics (Db : DB) (Sem: SEM Db) (Sql : SQL Db) (Ev : EV Db Sql).
       j_tb_sem d G s T ST ->
       j_btb_sem d G G0 btb Sbtb -> length s = length s' ->
       j_btb_sem d G (s'::G0) ((T,s')::btb) (fun Vl => cast _ _ e (Rel.times (ST Vl) (Sbtb Vl)))
-  with j_in_q_sem (d : Db.D) : forall G, prequery -> (env G -> bool) -> Prop :=
-  | jiqs_sel : forall G b tml btb c,
-      forall G0 Sbtb Sc Stml,
+  with j_btbl_sem (d : Db.D) : forall G G', list (list (pretb * Scm)) -> (env G -> Rel.R (list_sum (List.map (length (A:=Name)) G'))) -> Prop :=
+  | jbtbls_nil : forall G, j_btbl_sem d G List.nil List.nil (fun _ => Rel.Rone) 
+  | jbtbls_cons : forall G btb btbl,
+      forall G0 G1 Sbtb Sbtbl e,
       j_btb_sem d G G0 btb Sbtb ->
+      j_btbl_sem d (G0 ++ G) G1 btbl Sbtbl ->
+      j_btbl_sem d G (G1 ++ G0) (btb::btbl)
+        (fun h =>
+         let Rbtb := Sbtb h in
+         R_sum Rbtb (fun Vl => cast _ _ e (Rel.times (R_single Vl) (Sbtbl (Ev.env_app _ _ (Ev.env_of_tuple _ Vl) h)))))
+(*         let Rbtbl := Sbtbl h in
+         R_sum Rbtbl (fun Vl => cast _ _ e (Rel.times (Sbtb (Ev.env_app _  _ (Ev.env_of_tuple _ Vl) h)) (R_single Vl))))
+*)
+  with j_in_q_sem (d : Db.D) : forall G, prequery -> (env G -> bool) -> Prop :=
+  | jiqs_sel : forall G b tml btbl c,
+      forall G0 Sbtbl Sc Stml,
+      j_btbl_sem d G G0 btbl Sbtbl ->
       j_cond_sem d (G0++G) c Sc ->
       j_tml_sem (G0++G) (List.map fst tml) Stml ->
-      j_in_q_sem d G (select b tml btb c) 
-        (fun h => let S1 := Sbtb h in
+      j_in_q_sem d G (select b tml btbl c) 
+        (fun h => let S1 := Sbtbl h in
                   let p  := fun Vl => Sem.is_btrue (Sc (Ev.env_app _ _ (Ev.env_of_tuple G0 Vl) h)) in
                   let S2 := Rel.sel S1 p in
                   let f  := fun Vl => Stml (Ev.env_app _ _ (Ev.env_of_tuple G0 Vl) h) in
                   let S := Rel.sum S2 f
                   in 0 <? Rel.card (if b then Rel.flat S else S))
-  | jiqs_selstar : forall G b btb c,
-      forall G0 Sbtb Sc,
-      j_btb_sem d G G0 btb Sbtb ->
+  | jiqs_selstar : forall G b btbl c,
+      forall G0 Sbtbl Sc,
+      j_btbl_sem d G G0 btbl Sbtbl ->
       j_cond_sem d (G0++G) c Sc ->
-      j_in_q_sem d G (selstar b btb c) 
-        (fun h => let S1 := Sbtb h in
+      j_in_q_sem d G (selstar b btbl c) 
+        (fun h => let S1 := Sbtbl h in
                   let p  := fun Vl => Sem.is_btrue (Sc (Ev.env_app _ _ (Ev.env_of_tuple G0 Vl) h)) in
                   let S2 := Rel.sel S1 p in
 (*                  let f  := fun _ => Vector.nil Rel.V) in
@@ -684,9 +235,10 @@ no, we can simplify *)
   with jTs_ind_mut := Induction for j_tb_sem Sort Prop
   with jcs_ind_mut := Induction for j_cond_sem Sort Prop
   with jbTs_ind_mut := Induction for j_btb_sem Sort Prop
+  with jbTls_ind_mut := Induction for j_btbl_sem Sort Prop
   with jiqs_ind_mut := Induction for j_in_q_sem Sort Prop.
 
-  Combined Scheme j_sem_ind_mut from jqs_ind_mut, jTs_ind_mut, jcs_ind_mut, jbTs_ind_mut, jiqs_ind_mut.
+  Combined Scheme j_sem_ind_mut from jqs_ind_mut, jTs_ind_mut, jcs_ind_mut, jbTs_ind_mut, jbTls_ind_mut, jiqs_ind_mut.
 
 
   Derive Inversion j_q_sel_sem with (forall d G s b tml btb c Ssel, j_q_sem d G s (select b tml btb c) Ssel) Sort Prop.
@@ -697,6 +249,7 @@ no, we can simplify *)
   Derive Inversion j_tb_base_sem with (forall d G s x ST, j_tb_sem d G s (tbbase x) ST) Sort Prop.
   Derive Inversion j_tb_query_sem with (forall d G s q ST, j_tb_sem d G s (tbquery q) ST) Sort Prop.
   Derive Inversion j_cons_btb_sem with (forall d G G' T s tl Scons, j_btb_sem d G G' ((T,s)::tl) Scons) Sort Prop.
+  Derive Inversion j_cons_btbl_sem with (forall d G G' btb btbl Scons, j_btbl_sem d G G' (btb::btbl) Scons) Sort Prop.
   Derive Inversion j_iq_sel_sem with (forall d G b tml btb c Ssel, j_in_q_sem d G (select b tml btb c) Ssel) Sort Prop.
   Derive Inversion j_iq_selstar_sem with (forall d G b btb c Sss, j_in_q_sem d G (selstar b btb c) Sss) Sort Prop.
   Derive Inversion j_iq_union_sem with (forall d G b q1 q2 Sq, j_in_q_sem d G (qunion b q1 q2) Sq) Sort Prop.
@@ -720,12 +273,31 @@ no, we can simplify *)
     discriminate H5.
   Qed.
 
+  Lemma j_nil_btbl_sem :
+    forall d G G' Snil (P : Prop),
+       (forall (G0 G0': Ctx), G0 = G -> G0' = G' -> List.nil = G0' ->
+        (fun (_:Ev.env G) => Rel.Rone) ~= Snil -> P) ->
+       j_btbl_sem d G G' List.nil Snil -> P.
+  Proof.
+    intros.
+    enough (forall G0 G0' btbl0
+      (Snil0 : Ev.env G0 -> Rel.R (list_sum (List.map (length (A:=Name)) G0'))), 
+        j_btbl_sem d G0 G0' btbl0 Snil0 ->
+        G0 = G -> G0' = G' -> List.nil = btbl0 -> Snil0 ~= Snil -> P).
+    apply (H1 _ _ _ _ H0 eq_refl eq_refl eq_refl JMeq_refl).
+    intros G0 G0' btbl0 Snil0 H0'.
+    destruct H0'; intros. eapply H; auto. rewrite H1 in H4. exact H4.
+    discriminate H4.
+  Qed.
+
   Theorem j_sem_fun : forall d,
     (forall G s q Sq, j_q_sem d G s q Sq -> forall s0 Sq0, j_q_sem d G s0 q Sq0 -> s = s0 /\ Sq ~= Sq0) /\
     (forall G s T ST, j_tb_sem d G s T ST -> forall s0 ST0, j_tb_sem d G s0 T ST0 -> s = s0 /\ ST ~= ST0) /\
     (forall G c Sc, j_cond_sem d G c Sc -> forall Sc0, j_cond_sem d G c Sc0 -> Sc ~= Sc0) /\
     (forall G G' btb Sbtb, j_btb_sem d G G' btb Sbtb -> 
       forall G0' Sbtb0, j_btb_sem d G G0' btb Sbtb0 -> G' = G0' /\ Sbtb ~= Sbtb0) /\
+    (forall G G' btbl Sbtbl, j_btbl_sem d G G' btbl Sbtbl -> 
+      forall G0' Sbtbl0, j_btbl_sem d G G0' btbl Sbtbl0 -> G' = G0' /\ Sbtbl ~= Sbtbl0) /\
     (forall G q Sq, j_in_q_sem d G q Sq -> forall Sq0, j_in_q_sem d G q Sq0 -> Sq ~= Sq0).
   Proof.
     intro. apply j_sem_ind_mut.
@@ -734,25 +306,25 @@ no, we can simplify *)
       (* the Coq refiner generates an ill-typed term if we don't give enough parameters to this eapply *)
       eapply (j_q_sel_sem _ _ _ _ _ _ _ _ (fun _ _ s1 _ _ _ _ Ssel =>
         _ = s1 /\ (fun h =>
-        let S1 := Sbtb h in
+        let S1 := Sbtbl h in
         let p := fun Vl => is_btrue (Sc (Ev.env_app G0 G (Ev.env_of_tuple G0 Vl) h)) in
         let S2 := Rel.sel S1 p in
         let f := fun Vl => Stml (Ev.env_app G0 G (Ev.env_of_tuple G0 Vl) h) in
         let S := cast _ _ e (Rel.sum S2 f) in
         if b then Rel.flat S else S) ~= Ssel) _ H1). Unshelve.
       intros; simpl; subst. apply (existT_eq_elim H13); clear H13; intros; subst.
-      clear H3 H12. apply (existT_eq_elim (JMeq_eq H4)); clear H4; intros; subst.
-      clear H3. destruct (H _ _ H5); subst. pose (H11 := H0 _ H9); clearbody H11. 
+      clear H3. apply (existT_eq_elim (JMeq_eq H4)); clear H4; intros; subst.
+      clear H3. destruct (H _ _ H7); subst. pose (H11 := H0 _ H8); clearbody H11. 
       rewrite H4.
       rewrite H11.
-      replace e0 with e. replace Stml0 with Stml.
-      split; reflexivity. apply (Ev.j_tml_sem_fun _ _ _ j1 _ H10). apply UIP.
+      replace e1 with e. replace Stml0 with Stml.
+      split; reflexivity. apply (j_tml_sem_fun _ _ _ j1 _ H9). apply UIP.
     + intros. eapply (j_q_selstar_sem _ _ _ _ _ _ _ (fun _ _ _ _ _ _ _ => _) _ H1). Unshelve.
       intros; simpl; subst. apply (existT_eq_elim H12); clear H12; intros; subst.
-      clear H3 H11. apply (existT_eq_elim (JMeq_eq H4)); clear H4; intros; subst.
-      clear H3. destruct (H _ _ H6); subst. pose (H10 := H0 _ H8); clearbody H10. 
-      rewrite H4, H10. replace e0 with e. replace Stml0 with Stml.
-      split; reflexivity. apply (Ev.j_tml_sem_fun _ _ _ j1 _ H9). apply UIP.
+      clear H3. apply (existT_eq_elim (JMeq_eq H4)); clear H4; intros; subst.
+      clear H3. destruct (H _ _ H6); subst. pose (H10 := H0 _ H7); clearbody H10. 
+      rewrite H4, H10. replace e1 with e. replace Stml0 with Stml.
+      split; reflexivity. apply (j_tml_sem_fun _ _ _ j1 _ H8). apply UIP.
     + intros. eapply (j_q_union_sem _ _ _ _ _ _ _ (fun _ _ _ _ _ _ _ => _) _ H1). Unshelve.
       intros; simpl; subst. apply (existT_eq_elim H10); clear H10; intros; subst.
       clear H3 H2. apply (existT_eq_elim (JMeq_eq H5)); clear H5; intros; subst.
@@ -780,16 +352,16 @@ no, we can simplify *)
     + intros. inversion H. reflexivity.
     + intros. inversion H. reflexivity.
     + intros. inversion H. apply (existT_eq_elim H4); clear H4; intros; subst.
-      replace St0 with St. reflexivity. apply (Ev.j_tm_sem_fun _ _ _ j _ H2).
+      replace St0 with St. reflexivity. apply (j_tm_sem_fun _ _ _ j _ H2).
     + intros. inversion H. apply (existT_eq_elim H3); clear H3; intros; subst.
       apply (existT_eq_elim H5); clear H5; intros; subst. 
       replace e0 with (@eq_refl _ (length tml)).
       replace Stml0 with Stml. reflexivity.
-      apply (Ev.j_tml_sem_fun _ _ _ j _ H2). apply UIP.
+      apply (j_tml_sem_fun _ _ _ j _ H2). apply UIP.
     + intros. inversion H0. apply (existT_eq_elim H6); clear H6; intros; subst. clear H6.
       destruct (H _ _ H7). subst. rewrite H2.
       replace Stml0 with Stml. replace e'0 with e'. reflexivity.
-      apply UIP. apply (Ev.j_tml_sem_fun _ _ _ j _ H4).
+      apply UIP. apply (j_tml_sem_fun _ _ _ j _ H4).
     + intros. inversion H0. apply (existT_eq_elim H3); clear H3; intros; subst. clear H3.
       rewrite (H _ H4). reflexivity.
     + intros. inversion H1. apply (existT_eq_elim H5); clear H5; intros; subst.
@@ -806,10 +378,18 @@ no, we can simplify *)
       clear H11 H3. apply (existT_eq_elim (JMeq_eq H4)); clear H4; intros; subst.
       clear H3. destruct (H _ _ H6); subst. destruct (H0 _ _ H8); subst. intuition.
       rewrite H5. replace e with e1. reflexivity. apply UIP.
+    (* btbl *)
+    + intros. eapply (j_nil_btbl_sem _ _ _ _ _ _ H). Unshelve. simpl.
+      intros; simpl; subst. intuition.
+    + intros. eapply (j_cons_btbl_sem _ _ _ _ _ _ (fun _ _ _ _ _ _ => _) _ H1). Unshelve.
+      intros; simpl; subst. apply (existT_eq_elim H10); clear H10; intros; subst.
+      clear H9 H3. apply (existT_eq_elim (JMeq_eq H4)); clear H4; intros.
+      destruct (H _ _ H5); subst. destruct (H0 _ _ H7); subst; intuition.
+      clear H3. rewrite H6. replace e with e0. reflexivity. apply UIP.
     (* inner query *)
     + intros. eapply (j_iq_sel_sem _ _ _ _ _ _ _ (fun _ _ _ _ _ _ Ssel =>
         (fun h =>
-         let S1 := Sbtb h in
+         let S1 := Sbtbl h in
          let p := fun Vl => is_btrue (Sc (Ev.env_app G0 G (Ev.env_of_tuple G0 Vl) h)) in
          let S2 := Rel.sel S1 p in
          let f := fun Vl => Stml (Ev.env_app G0 G (Ev.env_of_tuple G0 Vl) h) in
@@ -818,7 +398,7 @@ no, we can simplify *)
       intros; simpl; subst. apply (existT_eq_elim H11); clear H11; intros; subst.
       clear H2 H3. destruct (H _ _ H4); subst. pose (H9 := H0 _ H7); clearbody H9. 
       rewrite H3, H9. replace Stml0 with Stml. reflexivity.
-      apply (Ev.j_tml_sem_fun _ _ _ j1 _ H8).
+      apply (j_tml_sem_fun _ _ _ j1 _ H8).
     + intros. eapply (j_iq_selstar_sem _ _ _ _ _ _ (fun _ _ _ _ _ _ => _) _ H1). Unshelve.
       intros; simpl; subst. apply (existT_eq_elim H9); clear H9; intros; subst.
       clear H2 H4. destruct (H _ _ H3); subst. pose (H7 := H0 _ H6); clearbody H7. 
@@ -844,18 +424,23 @@ no, we can simplify *)
     (forall G G' btb Sbtb, j_btb_sem d G G' btb Sbtb -> 
       forall G0 G0' btb0 Sbtb0, G = G0 -> btb = btb0 -> j_btb_sem d G0 G0' btb0 Sbtb0 -> 
       G' = G0' /\ Sbtb ~= Sbtb0) /\
+    (forall G G' btbl Sbtbl, j_btbl_sem d G G' btbl Sbtbl -> 
+      forall G0 G0' btbl0 Sbtbl0, G = G0 -> btbl = btbl0 -> j_btbl_sem d G0 G0' btbl0 Sbtbl0 -> 
+      G' = G0' /\ Sbtbl ~= Sbtbl0) /\
     (forall G q Sq, j_in_q_sem d G q Sq -> 
       forall G0 q0 Sq0, G = G0 -> q = q0 -> j_in_q_sem d G0 q0 Sq0 -> Sq ~= Sq0).
   Proof.
     intro. decompose [and] (j_sem_fun d). split.
-      intros. subst. apply (H _ _ _ _ H3 _ _ H7).
+      intros. subst. apply (H _ _ _ _ H4 _ _ H8).
     split.
-      intros. subst. apply (H1 _ _ _ _ H3 _ _ H7).
+      intros. subst. apply (H1 _ _ _ _ H4 _ _ H8).
     split.
-      intros. subst. apply (H0 _ _ _ H3 _ H7).
+      intros. subst. apply (H0 _ _ _ H4 _ H8).
     split.
-      intros. subst. apply (H2 _ _ _ _ H3 _ _ H7).
-    intros. subst. apply (H4 _ _ _ H3 _ H7).
+      intros. subst. apply (H2 _ _ _ _ H4 _ _ H8).
+    split.
+      intros. subst. apply (H3 _ _ _ _ H4 _ _ H8).
+    intros. subst. apply (H5 _ _ _ H4 _ H8).
   Qed.
 
   Corollary jT_sem_fun_dep : forall d G s T ST, j_tb_sem d G s T ST -> 
