AbstractRelation.v
@@ -10,6 +10,7 @@ Module Type REL.
   Parameter inter : forall n, R n -> R n -> R n.
   Parameter times : forall m n, R m -> R n -> R (m + n).
   Parameter sum   : forall m n, R m -> (T m -> T n) -> R n.
+  Parameter rsum  : forall m n, R m -> (T m -> R n) -> R n.
   Parameter sel   : forall n, R n -> (T n -> bool) -> R n.
   Parameter flat  : forall n, R n -> R n.
   Parameter supp  : forall n, R n -> list (T n).
@@ -20,6 +21,7 @@ Module Type REL.
   Implicit Arguments inter [n].
   Implicit Arguments times [m n].
   Implicit Arguments sum [m n].
+  Implicit Arguments rsum [m n].
   Implicit Arguments sel [n].
   Implicit Arguments flat [n].
   Implicit Arguments supp [n].
@@ -27,8 +29,13 @@ Module Type REL.
   Definition card := fun n S => memb (@sum n 0 S (fun _ => Vector.nil _)) (Vector.nil _).
   Implicit Arguments card [n].
 
-  Parameter Rnil : R 0.
+  Parameter Rnil : forall n, R n.
   Parameter Rone : R 0.
+  Parameter Rsingle : forall n, T n -> R n.
+
+  Implicit Arguments Rnil [n].
+  Implicit Arguments Rsingle [n].
+
   (* generalized cartesian product of m relations, each taken with its arity n *)
   Fixpoint prod (Rl : list { n : nat & R n }) 
     : R (list_sum (List.map (projT1 (P := fun n => R n)) Rl)) :=
@@ -46,16 +53,8 @@ Module Type REL.
   Hypothesis V_dec : forall (v w : V), {v = w} + {v <> w}.
   Hypothesis V_eqb_eq : forall (v w : V), V_eqb v w = true <-> v = w.
   Parameter T_dec : forall n, forall (x y : T n), {x = y} + {x <> y}.
-(*
-  Proof.
-    intros. eapply Vector.eq_dec. apply V_eqb_eq.
-  Qed.
-*)
+
   Parameter T_eqb_eq : forall n, forall (v w : T n), T_eqb v w = true <-> v = w.
-(*  Proof.
-    intros. eapply Vector.eqb_eq. apply V_eqb_eq.
-  Qed.
-*)
 
   Parameter p_fs : forall n, forall r : R n, forall t, memb r t > 0 -> List.In t (supp r).
   Parameter p_fs_r : forall n, forall r : R n, forall t, List.In t (supp r) -> memb r t > 0.
@@ -67,11 +66,15 @@ Module Type REL.
                       t = Vector.append t1 t2 -> memb (times r1 r2) t = memb r1 t1 * memb r2 t2.
   Parameter p_sum : forall m n, forall r : R m, forall f : T m -> T n, forall t, 
                     memb (sum r f) t = list_sum (List.map (memb r) (filter (fun x => T_eqb (f x) t) (supp r))).
+  Parameter p_rsum : forall m n, forall r : R m, forall f : T m -> R n, forall t,
+                    memb (rsum r f) t = list_sum (List.map (fun t0 => memb r t0 * memb (f t0) t) (supp r)).
   Parameter p_self : forall n, forall r : R n, forall p t, p t = false -> memb (sel r p) t = 0.
   Parameter p_selt : forall n, forall r : R n, forall p t, p t = true -> memb (sel r p) t = memb r t.
   Parameter p_flat : forall n, forall r : R n, forall t, memb (flat r) t = flatnat (memb r t).
-  Parameter p_nil : forall r, memb Rnil r = 0.
-  Parameter p_one : forall r, memb Rone r = 1.
+  Parameter p_nil : forall n (t : T n), memb Rnil t = 0.
+  Parameter p_one : forall t, memb Rone t = 1.
+  Parameter p_single : forall n (t : T n), memb (Rsingle t) t = 1.
+  Parameter p_single_neq : forall n (t1 t2 : T n), t1 <> t2 -> memb (Rsingle t1) t2 = 0.
 
   Parameter p_ext : forall n, forall r s : R n, (forall t, memb r t = memb s t) -> r = s.
 
